upd

Earley_List.thy
@@ -2418,6 +2418,7 @@ fun combinations :: "'a set list \<Rightarrow> 'a list set" where
 | "combinations (xs#xss) = \<Union> ((\<lambda>x. (\<lambda>c. x # c) ` (combinations xss))` xs)"
 
 value "combinations [{1,2},{3},{4,5::nat}]"
+value "combinations ([{1,2},{3}] @ [{4::nat,5}])"
 
 fun trees :: "'a forest \<Rightarrow> 'a tree set" where
   "trees (FLeaf a) = {Leaf a}"
@@ -2563,6 +2564,8 @@ qed simp
 lemma sound_ptrs_bin_upd: \<comment>\<open>TODO\<close>
   assumes "sound_ptrs inp bs" "k < length bs" "es = bs!k" "distinct (items es)"
   assumes "sound_null_ptr e" "sound_pre_ptr inp bs k e" "sound_prered_ptr bs k e"
+(*  assumes "\<forall>k' pre red reds i red' reds'. i < length es \<longrightarrow> PreRed (k', pre, red) reds = pointer (es!i) \<longrightarrow> item e = item (es!i) \<longrightarrow>
+    PreRed (k', pre, red') reds' = pointer e" *)
   shows "sound_ptrs inp (bs[k := bin_upd e es])"
   unfolding sound_ptrs_def
 proof (standard, standard, standard)
@@ -2926,6 +2929,384 @@ proof (induction bs inp k i rule: build_tree'.induct)
     case Null
     hence 0: "build_tree' bs inp k i = Branch (item_rule_head (item ?e)) []"
       by simp
+    have "predicts (item ?e)"
+      using Null "1.prems"(2,3,4) nth_mem unfolding sound_ptrs_def sound_null_ptr_def by blast
+    hence "item_dot (item ?e) = 0"
+      unfolding predicts_def by blast
+    thus ?thesis
+      using 0 by simp
+  next
+    case Pre
+    then obtain pre where pre: "pointer ?e = Pre pre"
+      by blast
+    obtain N ts where node: "build_tree' bs inp (k-1) pre = Branch N ts"
+      by (meson ex_Branch_build_tree')
+    hence simp: "build_tree' bs inp k i = Branch N (ts @ [Leaf (inp!(k-1))])"
+      using pre by simp
+    have bounds: "pre < length (bs!(k-1))"
+      using "1.prems"(2,3,4) pre unfolding sound_ptrs_def sound_pre_ptr_def by (metis nth_mem)
+    have scans: "scans inp k (item (bs!(k-1)!pre)) (item (bs!k!i))"
+      using "1.prems"(2,3,4) pre unfolding sound_ptrs_def sound_pre_ptr_def by simp
+    have IH: "wf_item_tree cfg (item (bs!(k-1)!pre)) (build_tree' bs inp (k-1) pre)"
+      using "1.IH"(1) pre "1.prems"(1,2,3,4) bounds by simp
+    hence *: 
+      "item_rule_head (item (bs!(k-1)!pre)) = item_rule_head (item (bs!k!i))"
+      "item_rule_body (item (bs!(k-1)!pre)) = item_rule_body (item (bs!k!i))"
+      "item_dot (item (bs!(k-1)!pre)) + 1 = item_dot (item (bs!k!i))"
+      "next_symbol (item (bs!(k-1)!pre)) = Some (inp!(k-1))"
+      using scans unfolding scans_def inc_item_def by (simp_all add: item_rule_head_def item_rule_body_def)
+    have "map root_tree (ts @ [Leaf (inp!(k-1))]) = map root_tree ts @ [inp!(k-1)]"
+      by simp
+    also have "... = take (item_dot (item (bs!(k-1)!pre))) (item_rule_body (item (bs!(k-1)!pre))) @ [inp!(k-1)]"
+      using IH node by simp
+    also have "... = take (item_dot (item (bs!(k-1)!pre))) (item_rule_body (item (bs!k!i))) @ [inp!(k-1)]"
+      using *(2) by simp
+    also have "... = take (item_dot (item (bs!k!i))) (item_rule_body (item (bs!k!i)))"
+      using *(2-4) by (auto simp: next_symbol_def is_complete_def split: if_splits; metis leI take_Suc_conv_app_nth)
+    finally show ?thesis
+      using *(1) IH node simp by simp
+  next
+    case PreRed
+    then obtain k' pre red ps where prered: "pointer ?e = PreRed (k', pre, red) ps"
+      by auto
+    obtain N ts where node: "build_tree' bs inp k' pre = Branch N ts"
+      by (meson ex_Branch_build_tree')
+    hence simp: "build_tree' bs inp k i = Branch N (ts @ [build_tree' bs inp k red])"
+      using prered by simp
+    have bounds: "k' < k" "pre < length (bs!k')" "red < length (bs!k)"
+      using "1.prems" prered unfolding sound_ptrs_def sound_prered_ptr_def by (metis list.set_intros(1) nth_mem)+
+    have completes: "completes k (item (bs!k'!pre)) (item (bs!k!i)) (item (bs!k!red))"
+      using "1.prems" prered unfolding sound_ptrs_def sound_prered_ptr_def by (metis list.set_intros(1) nth_mem)
+    have IH_pre: "wf_item_tree cfg (item (bs!k'!pre)) (build_tree' bs inp k' pre)"
+      using "1.IH"(2) "1.prems"(1-4) bounds prered by simp
+    have IH_red: "wf_item_tree cfg (item (bs!k!red)) (build_tree' bs inp k red)"
+      using "1.IH"(3) "1.prems" bounds prered node by simp
+    have *: 
+      "item_rule_head (item (bs!k'!pre)) = item_rule_head (item (bs!k!i))"
+      "item_rule_body (item (bs!k'!pre)) = item_rule_body (item (bs!k!i))"
+      "item_dot (item (bs!k'!pre)) + 1 = item_dot (item (bs!k!i))"
+      "next_symbol (item (bs!k'!pre)) = Some (item_rule_head (item (bs!k!red)))"
+      "is_complete (item (bs!k!red))"
+      using completes unfolding completes_def inc_item_def
+      by (auto simp: item_rule_head_def item_rule_body_def is_complete_def)
+    have "map root_tree (ts @ [build_tree' bs inp k red]) = map root_tree ts @ [root_tree (build_tree' bs inp k red)]"
+      by simp
+    also have "... = take (item_dot (item (bs!k'!pre))) (item_rule_body (item (bs!k'!pre))) @ [root_tree (build_tree' bs inp k red)]"
+      using IH_pre node by force
+    also have "... = take (item_dot (item (bs!k'!pre))) (item_rule_body (item (bs!k'!pre))) @ [item_rule_head (item (bs!k!red))]"
+      using IH_red ex_Branch_build_tree' by (metis root_tree.simps(2) wf_item_tree.simps(2))
+    also have "... = take (item_dot (item (bs!k!i))) (item_rule_body (item (bs!k!i)))"
+      using * by (auto simp: next_symbol_def is_complete_def split: if_splits; metis leI take_Suc_conv_app_nth)
+    finally have 0: "map root_tree (ts @ [build_tree' bs inp k red]) = take (item_dot (item (bs!k!i))) (item_rule_body (item (bs!k!i)))" .
+    have wf: "wf_item cfg inp (item (bs!k!red))"
+      using "1.prems" bounds(3) unfolding wf_bins_def wf_bin_def wf_bin_items_def by (simp add: items_def)
+    obtain N' ts' where node': "build_tree' bs inp k red = Branch N' ts'"
+      by (meson ex_Branch_build_tree')
+    hence "N' = item_rule_head (item (bs!k!red))"
+          "map root_tree ts' = item_rule_body (item (bs!k!red))"
+      using IH_red *(5) by (auto simp: is_complete_def)
+    hence "\<exists>r \<in> set (\<RR> cfg). N' = rule_head r \<and> map root_tree ts' = rule_body r"
+      using wf unfolding wf_item_def item_rule_body_def item_rule_head_def by auto
+    hence 1: "wf_rule_tree cfg (build_tree' bs inp k red)"
+      using IH_red node' by simp
+    show ?thesis
+      using *(1) 0 1 IH_pre node simp by simp
+  qed
+qed
+
+lemma wf_yield_tree_build_tree':
+  assumes "wf_bins cfg inp bs"
+  assumes "sound_ptrs inp bs"
+  assumes "k < length bs" "i < length (bs!k)" "k \<le> length inp"
+  shows "wf_yield_tree inp (item (bs!k!i)) (build_tree' bs inp k i)"
+  using assms
+proof (induction bs inp k i rule: build_tree'.induct)
+  case (1 bs inp k i)
+  let ?e = "bs!k!i"
+  consider (Null) "pointer ?e = Null" | (Pre) "\<exists>pre. pointer ?e = Pre pre" | (PreRed) "\<exists>p ps. pointer ?e = PreRed p ps"
+    by (meson PreRed pointer.exhaust)
+  thus ?case
+  proof cases
+    case Null
+    hence simp: "build_tree' bs inp k i = Branch (item_rule_head (item ?e)) []"
+      by simp
+    have "predicts (item ?e)"
+      using Null "1.prems"(2,3,4) unfolding sound_ptrs_def sound_null_ptr_def by simp
+    hence "item_origin (item ?e) = item_end (item ?e)"
+      unfolding predicts_def by blast
+    thus ?thesis
+      unfolding wf_yield_tree_def using simp by (simp add: slice_empty)
+  next
+    case Pre
+    then obtain pre where pre: "pointer ?e = Pre pre"
+      by blast
+    obtain N ts where node: "build_tree' bs inp (k-1) pre = Branch N ts"
+      by (meson ex_Branch_build_tree')
+    hence simp: "build_tree' bs inp k i = Branch N (ts @ [Leaf (inp!(k-1))])"
+      using pre by simp
+    have bounds: "k > 0" "pre < length (bs!(k-1))"
+      using "1.prems"(2,3,4) pre unfolding sound_ptrs_def sound_pre_ptr_def by (metis nth_mem)+
+    have scans: "scans inp k (item (bs!(k-1)!pre)) (item (bs!k!i))"
+      using "1.prems"(2,3,4) pre unfolding sound_ptrs_def sound_pre_ptr_def by simp
+    have IH: "wf_yield_tree inp (item (bs!(k-1)!pre)) (build_tree' bs inp (k-1) pre)"
+      using "1.IH"(1) pre "1.prems"(1,2,3,5) bounds by simp
+    have wf: 
+      "item_origin (item (bs!(k-1)!pre)) \<le> item_end (item (bs!(k-1)!pre))"
+      "item_end (item (bs!(k-1)!pre)) = k-1"
+      "item_end (item (bs!k!i)) = k"
+      using "1.prems"(1,3,4) bounds unfolding wf_bins_def wf_bin_def wf_bin_items_def items_def wf_item_def
+      by (auto, meson less_imp_diff_less nth_mem)
+    have "yield_tree (build_tree' bs inp k i) = concat (map yield_tree (ts @ [Leaf (inp!(k-1))]))"
+      using simp by simp
+    also have "... = concat (map yield_tree ts) @ [inp!(k-1)]"
+      by simp
+    also have "... = slice (item_origin (item (bs!(k-1)!pre))) (item_end (item (bs!(k-1)!pre))) inp @ [inp!(k-1)]"
+      using node IH by (simp add: wf_yield_tree_def)
+    also have "... = slice (item_origin (item (bs!(k-1)!pre))) (item_end (item (bs!(k-1)!pre)) + 1) inp"
+      using slice_append_nth wf "1.prems"(5) \<open>k > 0\<close> by (metis Suc_diff_1 linorder_not_le not_less_eq)
+    also have "... = slice (item_origin (item ?e)) (item_end (item (bs!(k-1)!pre)) + 1) inp"
+      using scans unfolding scans_def inc_item_def by simp
+    also have "... = slice (item_origin (item ?e)) k inp"
+      using scans wf unfolding scans_def by (metis Suc_diff_1 Suc_eq_plus1 bounds(1))
+    also have "... = slice (item_origin (item ?e)) (item_end (item ?e)) inp"
+      using wf by auto
+    finally show ?thesis
+      using wf_yield_tree_def by blast
+  next
+    case PreRed
+    then obtain k' pre red ps where prered: "pointer ?e = PreRed (k', pre, red) ps"
+      by auto
+    obtain N ts where node: "build_tree' bs inp k' pre = Branch N ts"
+      by (meson ex_Branch_build_tree')
+    hence simp: "build_tree' bs inp k i = Branch N (ts @ [build_tree' bs inp k red])"
+      using prered by simp
+    have bounds: "k' < k" "pre < length (bs!k')" "red < length (bs!k)"
+      using "1.prems"(2,3,4) prered unfolding sound_ptrs_def sound_prered_ptr_def by (metis list.set_intros(1) nth_mem)+
+    have completes: "completes k (item (bs!k'!pre)) (item (bs!k!i)) (item (bs!k!red))"
+      using "1.prems"(2,3,4) prered unfolding sound_ptrs_def sound_prered_ptr_def by (metis list.set_intros(1) nth_mem)
+    have IH_pre: "wf_yield_tree inp (item (bs!k'!pre)) (build_tree' bs inp k' pre)"
+      using "1.IH"(2) "1.prems"(1-3,5) bounds prered by simp
+    have IH_red: "wf_yield_tree inp (item (bs!k!red)) (build_tree' bs inp k red)"
+      using "1.IH"(3) "1.prems"(1-5) bounds prered node by simp
+    have wf1: 
+      "item_origin (item (bs!k'!pre)) \<le> item_end (item (bs!k'!pre))"
+      "item_origin (item (bs!k!red)) \<le> item_end (item (bs!k!red))"
+      using "1.prems"(1,3,4) bounds unfolding wf_bins_def wf_bin_def wf_bin_items_def items_def wf_item_def
+      by (metis length_map nth_map nth_mem order_less_trans)+
+    have wf2:
+      "item_end (item (bs!k!red)) = k"
+      "item_end (item (bs!k!i)) = k"
+      using "1.prems"(1,3,4) bounds unfolding wf_bins_def wf_bin_def wf_bin_items_def items_def by simp_all
+    have "yield_tree (build_tree' bs inp k i) = concat (map yield_tree (ts @ [build_tree' bs inp k red]))"
+      using simp by simp
+    also have "... = concat (map yield_tree ts) @ yield_tree (build_tree' bs inp k red)"
+      by simp
+    also have "... = slice (item_origin (item (bs!k'!pre))) (item_end (item (bs!k'!pre))) inp @ 
+      slice (item_origin (item (bs!k!red))) (item_end (item (bs!k!red))) inp"
+      using IH_pre IH_red by (simp add: node wf_yield_tree_def)
+    also have "... = slice (item_origin (item (bs!k'!pre))) (item_end (item (bs!k!red))) inp"
+      using slice_concat wf1 completes_def completes by (metis (no_types, lifting))
+    also have "... = slice (item_origin (item ?e)) (item_end (item (bs!k!red))) inp"
+      using completes unfolding completes_def inc_item_def by simp
+    also have "... = slice (item_origin (item ?e)) (item_end (item ?e)) inp"
+      using wf2 by simp
+    finally show ?thesis
+      using wf_yield_tree_def by blast
+  qed
+qed
+
+theorem build_tree_Some_wf_rule_tree:
+  assumes "wf_bins cfg inp bs" "sound_ptrs inp bs" "length bs = length inp + 1"
+  assumes "Some t = build_tree cfg inp bs"
+  shows "wf_rule_tree cfg t \<and> root_tree t = \<SS> cfg \<and> yield_tree t = inp"
+proof -
+  let ?k = "length bs - 1"
+  obtain x i xs where *: "filter_with_index (is_finished cfg inp) (items (bs!?k)) = (x,i)#xs"
+    using assms(4) unfolding build_tree_def by (auto simp: Let_def split: list.splits)
+  have k: "?k < length bs" "?k \<le> length inp"
+    using assms(3) by simp_all
+  have i: "i < length (bs ! ?k)"
+    using index_filter_with_index_lt_length * items_def by (metis length_map list.set_intros(1))
+  have x: "x = item (bs!?k!i)"
+    using * i filter_with_index_nth items_def nth_map by (metis list.set_intros(1))
+  have finished: "is_finished cfg inp x"
+    using * filter_with_index_P by (metis list.set_intros(1))
+  hence wf_item_rule: "wf_item_tree cfg x (build_tree' bs inp ?k i)"
+    using wf_item_tree_build_tree' assms(1,2) i k(1) x by blast
+  have wf_item: "wf_item cfg inp (item (bs!?k!i))"
+    using k(1) i assms(1) unfolding wf_bins_def wf_bin_def wf_bin_items_def by (simp add: items_def)
+  obtain N ts where node: "build_tree' bs inp ?k i = Branch N ts"
+    by (meson ex_Branch_build_tree')
+  hence "N = item_rule_head x"
+    "map root_tree ts = item_rule_body x"
+    using finished wf_item_rule by (auto simp: is_finished_def is_complete_def)
+  hence "\<exists>r \<in> set (\<RR> cfg). N = rule_head r \<and> map root_tree ts = rule_body r"
+    using wf_item x unfolding wf_item_def item_rule_body_def item_rule_head_def by blast
+  hence wf_rule: "wf_rule_tree cfg (build_tree' bs inp ?k i)"
+    using wf_item_rule node by simp
+  have root: "root_tree (build_tree' bs inp ?k i) = \<SS> cfg"
+    using finished node \<open>N = item_rule_head x\<close> by (auto simp: is_finished_def)
+  have "yield_tree (build_tree' bs inp ?k i) = slice (item_origin (item (bs!?k!i))) (item_end (item (bs!?k!i))) inp"
+    using k i assms(1,2,3) wf_yield_tree_build_tree' wf_yield_tree_def by blast
+  hence yield: "yield_tree (build_tree' bs inp ?k i) = inp"
+    using finished x unfolding is_finished_def by simp
+  show ?thesis
+    using * wf_rule root yield assms(4) unfolding build_tree_def by simp
+qed
+
+corollary build_tree_Some_wf_rule_tree_\<II>_it:
+  assumes "wf_cfg cfg" "nonempty_derives cfg" "Some t = build_tree cfg inp (\<II>_it cfg inp)"
+  shows "wf_rule_tree cfg t \<and> root_tree t = \<SS> cfg \<and> yield_tree t = inp"
+  using assms build_tree_Some_wf_rule_tree wf_bins_\<II>_it sound_ptrs_\<II>_it \<II>_it_def
+    length_\<I>_it length_bins_Init_it by (metis nle_le)
+
+theorem build_tree_Some_\<II>_it:
+  assumes "wf_cfg cfg" "is_word cfg inp" "nonempty_derives cfg"
+  shows "(\<exists>t. Some t = build_tree cfg inp (\<II>_it cfg inp)) \<longleftrightarrow> derives cfg [\<SS> cfg] inp" (is "?L \<longleftrightarrow> ?R")
+proof standard
+  assume *: ?L
+  let ?k = "length (\<II>_it cfg inp) - 1"
+  obtain t where "Some t = build_tree cfg inp (\<II>_it cfg inp)"
+    using * by blast
+  then obtain x i xs where *: "filter_with_index (is_finished cfg inp) (items ((\<II>_it cfg inp)!?k)) = (x,i)#xs"
+    unfolding build_tree_def by (auto simp: Let_def split: list.splits)
+  have k: "?k < length (\<II>_it cfg inp)" "?k \<le> length inp"
+    by (simp_all add: \<II>_it_def assms(1))
+  have i: "i < length ((\<II>_it cfg inp) ! ?k)"
+    using index_filter_with_index_lt_length * items_def by (metis length_map list.set_intros(1))
+  have x: "x = item ((\<II>_it cfg inp)!?k!i)"
+    using * i filter_with_index_nth items_def nth_map by (metis list.set_intros(1))
+  have finished: "is_finished cfg inp x"
+    using * filter_with_index_P by (metis list.set_intros(1))
+  moreover have "x \<in> set (items ((\<II>_it cfg inp) ! ?k))"
+    using x by (auto simp: items_def; metis One_nat_def i imageI nth_mem)
+  ultimately have "(\<exists>x \<in> set (items ((\<II>_it cfg inp) ! length inp)). is_finished cfg inp x)"
+    by (metis assms(1) is_finished_def k(1) wf_bins_\<II>_it wf_bins_kth_bin)    
+  hence "earley_recognized_it (\<II>_it cfg inp) cfg inp"
+    using earley_recognized_it_def by blast
+  thus ?R
+    using correctness_list assms by blast
+next
+  assume ?R
+  hence "earley_recognized_it (\<II>_it cfg inp) cfg inp"
+    using assms(1) assms(2) assms(3) correctness_list by blast
+  hence "(\<exists>x\<in>set (items ((\<II>_it cfg inp) ! length inp)). is_finished cfg inp x)"
+    using earley_recognized_it_def by blast
+  hence "(\<exists>x\<in>set (items ((\<II>_it cfg inp) ! (length (\<II>_it cfg inp) - 1))). is_finished cfg inp x)"
+    by (simp add: \<II>_it_def assms(1))
+  hence "\<exists>x i xs. filter_with_index (is_finished cfg inp) (items ((\<II>_it cfg inp)! (length (\<II>_it cfg inp) - 1))) = (x,i)#xs"
+    using filter_with_index_cong_filter list.exhaust list.simps(8) prod.collapse by (metis empty_filter_conv)
+  thus ?L
+    by (auto simp: build_tree_def)
+qed
+
+subsection \<open>Parse forest lemmas\<close>
+
+function build_forest' :: "'a bins \<Rightarrow> 'a sentence \<Rightarrow> nat \<Rightarrow> nat \<Rightarrow> 'a forest" where
+  "build_forest' bs inp k i = (
+    let e = bs!k!i in (
+    case pointer e of
+      Null \<Rightarrow> FBranch (item_rule_head (item e)) [] \<comment>\<open>start building sub-forest\<close>
+    | Pre pre \<Rightarrow> ( \<comment>\<open>add sub-forest starting from terminal\<close>
+      case build_forest' bs inp (k-1) pre of
+        FBranch N fss \<Rightarrow> FBranch N (fss @ [[FLeaf (inp!(k-1))]])
+      | _ \<Rightarrow> undefined) \<comment>\<open>impossible case\<close>
+    | PreRed (k', pre, red) reds \<Rightarrow> ( \<comment>\<open>add sub-forest starting from non-terminal\<close>
+      case build_forest' bs inp k' pre of
+        FBranch N fss \<Rightarrow> FBranch N (fss @ [map (\<lambda>r. build_forest' bs inp k r) (red#reds)])
+      | _ \<Rightarrow> undefined) \<comment>\<open>impossible case\<close>
+    ))"
+  by pat_completeness auto
+termination sorry
+
+declare build_forest'.simps [simp del]
+
+definition build_forest :: "'a cfg \<Rightarrow> 'a sentence \<Rightarrow> 'a bins \<Rightarrow> 'a forest list" where
+  "build_forest cfg inp bs = (
+    let k = length bs - 1 in
+    let finished = filter_with_index (\<lambda>x. is_finished cfg inp x) (items (bs!k)) in
+    map (\<lambda>(_, i). build_forest' bs inp k i) finished
+  )"
+
+lemma build_forest'_simps[simp]:
+  "e = bs!k!i \<Longrightarrow> pointer e = Null \<Longrightarrow> build_forest' bs inp k i = FBranch (item_rule_head (item e)) []"
+  "e = bs!k!i \<Longrightarrow> pointer e = Pre pre \<Longrightarrow> build_forest' bs inp (k-1) pre = FBranch N fss \<Longrightarrow> 
+    build_forest' bs inp k i = FBranch N (fss @ [[FLeaf (inp!(k-1))]])"
+  "e = bs!k!i \<Longrightarrow> pointer e = PreRed (k', pre, red) reds \<Longrightarrow> build_forest' bs inp k' pre = FBranch N fss \<Longrightarrow>
+    build_forest' bs inp k i = FBranch N (fss @ [map (\<lambda>r. build_forest' bs inp k r) (red#reds)])"
+  by (auto simp: build_forest'.simps Let_def)
+
+lemma ex_Branch_build_forest':
+  "\<exists>N fss. build_forest' bs inp k i = FBranch N fss"
+  apply (induction bs inp k i rule: build_forest'.induct)
+  apply (subst build_forest'.simps)
+  apply (auto simp: Let_def split: list.splits forest.splits pointer.splits)
+  by (metis forest.distinct(1))+
+
+lemma nex_Leaf_build_forest':
+  "\<nexists>a. build_forest' bs inp k i = FLeaf a"
+  using ex_Branch_build_forest' by (metis forest.distinct(1))
+
+lemma combinations_singleton:
+  "combinations ([xs]) = { [x] | x. x \<in> xs }"
+  by auto
+
+lemma combinations_append:
+  "combinations (xss @ yss) = { xs @ ys | xs ys. xs \<in> combinations xss \<and> ys \<in> combinations yss }"
+  apply (induction xss)
+  apply (auto intro!: append_Cons imageI)
+  by (metis (no_types, opaque_lifting) append_Cons imageI)
+
+lemma combinations_append_singleton:
+  "combinations (xss @ [ys]) = { xs @ [y] | xs y. xs \<in> combinations xss \<and> y \<in> ys }"
+  apply (subst combinations_append)
+  apply (subst combinations_singleton)
+  by blast
+
+lemma combinations_append_single_singleton:
+  "combinations (xss @ [{y}]) = { xs @ [y] | xs. xs \<in> combinations xss }"
+  apply (subst combinations_append_singleton)
+  by auto
+
+lemma trees_append:
+  "trees (FBranch N (xss @ yss)) = (
+    let xtss = map (\<lambda>xs. \<Union>((\<lambda>x. trees x) ` (set xs))) xss in
+    let ytss = map (\<lambda>ys. \<Union>((\<lambda>y. trees y) ` (set ys))) yss in
+    (\<lambda>ts. Branch N ts) ` { xs @ ys | xs ys. xs \<in> combinations xtss \<and> ys \<in> combinations ytss })"
+  using combinations_append by (metis map_append trees.simps(2))
+
+lemma trees_append_singleton:
+  "trees (FBranch N (xss @ [ys])) = (
+    let xtss = map (\<lambda>xs. \<Union>((\<lambda>x. trees x) ` (set xs))) xss in
+    let ytss = [\<Union>((\<lambda>y. trees y) ` (set ys))] in
+    (\<lambda>ts. Branch N ts) ` { xs @ ys | xs ys. xs \<in> combinations xtss \<and> ys \<in> combinations ytss })"
+  by (subst trees_append, simp)
+
+lemma trees_append_single_singleton:
+  "trees (FBranch N (xss @ [[y]])) = (
+    let xtss = map (\<lambda>xs. \<Union>((\<lambda>x. trees x) ` (set xs))) xss in
+    (\<lambda>ts. Branch N ts) ` { xs @ ys | xs ys. xs \<in> combinations xtss \<and> ys \<in> { [t] | t. t \<in> trees y } })"
+  by (subst trees_append_singleton, auto)
+  
+lemma wf_item_tree_build_forest':
+  assumes "wf_bins cfg inp bs"
+  assumes "sound_ptrs inp bs"
+  assumes "k < length bs" "i < length (bs!k)"
+  assumes "t \<in> trees (build_forest' bs inp k i)"
+  shows "wf_item_tree cfg (item (bs!k!i)) t"
+  using assms
+proof (induction bs inp k i rule: build_forest'.induct)
+  case (1 bs inp k i)
+  let ?e = "bs!k!i"
+  consider (Null) "pointer ?e = Null" | (Pre) "\<exists>pre. pointer ?e = Pre pre" | (PreRed) "\<exists>p ps. pointer ?e = PreRed p ps"
+    by (meson PreRed pointer.exhaust)
+  thus ?case
+  proof cases
+    case Null
+    hence "build_forest' bs inp k i = FBranch (item_rule_head (item ?e)) []"
+      by simp
+    hence 0: "t = Branch (item_rule_head (item ?e)) []"
+      using "1.prems"(5) by force
     have "predicts (item ?e)"
       using Null "1.prems"(2,3,4) nth_mem unfolding sound_ptrs_def sound_null_ptr_def by blast
     hence "item_dot (item ?e) = 0"
